### 欧拉公式

$$
e^{ix} = cos x \ + i\ sin x
$$

证明使用泰勒展开，这里不写

推论：
$$
\begin{aligned}
cosx &= \frac{e^{ix}+e^{-ix}}{2}
\\
sinx &= \frac{e^{ix}-e^{-ix}}{2i}
\end{aligned}
$$

### 和差角

#### 证明

$$
\begin{aligned}
cos(\alpha + \beta) &= \frac{e^{i(\alpha + \beta)} + e^{-i(\alpha + \beta)}}{2}
\\
&= \frac{1}{2} (e^{i\alpha}e^{i\beta} + e^{-i\alpha}e^{-i\beta})
\\
&= \frac{1}{2} [ (cos\alpha+isin\alpha)(cos\beta+isin\beta) + (cos\alpha-isin\alpha)(cos\beta-isin\beta) ]
\\
&= \frac{1}{2} (cos\alpha cos\beta + icos\alpha sin\beta + isin\alpha cos\beta - sin\alpha sin\beta + cos\alpha cos\beta - i cos\alpha sin\beta - isin\alpha cos\beta - sin \alpha sin \beta)
\\
&= cos\alpha cos\beta - sin \alpha sin \beta
\\
~
\\
sin(\alpha + \beta) &= \frac{e^{i(\alpha + \beta)}-e^{-i(\alpha + \beta)}}{2i}
\\
&= \frac{1}{2i} (e^{i\alpha}e^{i\beta} - e^{-i\alpha}e^{-i\beta})
\\
&= \frac{1}{2i} [ (cos\alpha+isin\alpha)(cos\beta+isin\beta) - (cos\alpha-isin\alpha)(cos\beta-isin\beta) ]
\\
&= \frac{1}{2i} (cos\alpha cos\beta + icos\alpha sin\beta + isin\alpha cos\beta - sin\alpha sin\beta - cos\alpha cos\beta + i cos\alpha sin\beta + isin\alpha cos\beta + sin \alpha sin \beta)
\\
&= sin \alpha cos \beta + sin \beta cos \alpha
\end{aligned}
$$

可以由上述两式推导差角形式
$$
\begin{aligned}
cos(\alpha - \beta) &= cos(\alpha + (-\beta)) = cos\alpha \ cos \beta + sin \alpha \ sin \beta
\\
sin(\alpha - \beta) &= cos(\alpha + (-\beta)) = sin \alpha \ cos \beta - sin \beta cos \alpha
\end{aligned}
$$

#### 总结

$$
\begin{aligned}
cos(\alpha + \beta) &= cos\alpha \ cos\beta - sin \alpha \ sin \beta
\\
cos(\alpha - \beta) &= cos\alpha \ cos \beta + sin \alpha \ sin \beta
\\
sin(\alpha + \beta) &= sin \alpha \ cos \beta + sin \beta \ cos \alpha
\\
sin(\alpha - \beta) &= sin \alpha \ cos \beta - sin \beta \ cos \alpha
\end{aligned}
$$

### 和差化积

#### 证明

$$
\begin{aligned}
sin \alpha &= sin(\frac{\alpha + \beta}{2} + \frac{\alpha - \beta}{2})
\\
&= sin(\frac{\alpha + \beta}{2}) cos(\frac{\alpha - \beta}{2}) + sin(\frac{\alpha - \beta}{2}) cos(\frac{\alpha + \beta}{2})
\\
~
\\
cos \alpha &= cos(\frac{\alpha + \beta}{2} + \frac{\alpha - \beta}{2})
\\
&= cos(\frac{\alpha + \beta}{2}) cos(\frac{\alpha - \beta}{2}) - sin(\frac{\alpha - \beta}{2}) sin(\frac{\alpha + \beta}{2})
\end{aligned}
$$

#### 总结

$$
\begin{aligned}
sin \alpha + sin \beta &= 2 sin(\frac{\alpha + \beta}{2}) cos(\frac{\alpha - \beta}{2})
\\
sin \alpha - sin \beta &= 2 sin(\frac{\alpha - \beta}{2}) cos(\frac{\alpha + \beta}{2})
\\
cos \alpha + cos \beta &= 2 cos(\frac{\alpha + \beta}{2}) cos(\frac{\alpha - \beta}{2})
\\
cos \alpha - cos \beta &= -2 sin(\frac{\alpha + \beta}{2}) sin(\frac{\alpha - \beta}{2})
\end{aligned}
$$

### 积化和差

证明比较简单，和差角公式的加减而已，略
$$
\begin{aligned}
cos\alpha \ cos\beta &= \frac{1}{2} [cos(\alpha + \beta) + cos(\alpha - \beta)]
\\
sin \alpha \ sin \beta &= \frac{1}{2} [cos(\alpha - \beta) + cos(\alpha + \beta)]
\\
sin\alpha \ cos\beta &= \frac{1}{2} [sin(\alpha + \beta) + sin(\alpha - \beta)]
\\
cos\alpha \ sin\beta &= \frac{1}{2} [sin(\alpha + \beta) - sin(\alpha - \beta)]
\end{aligned}
$$
